cedar-lean/Cedar/Thm/Validation/WellTyped/LitVar.lean
@@ -15,6 +15,7 @@
 -/
 import Cedar.Validation.TypedExpr
 import Cedar.Thm.Validation.WellTyped.Definition
+import Cedar.Thm.Validation.WellTyped.TypeLifting
 import Cedar.Thm.Validation
 import Cedar.Spec
 
@@ -48,8 +49,7 @@ theorem typechecked_is_well_typed_after_lifting_lit {p : Prim} {c₁ c₂ : Capa
       rcases h₃ with ⟨h₃, _⟩
       simp only [← h₃, TypedExpr.liftBoolTypes, CedarType.liftBoolTypes]
       rename_i uid h₄ _
-      sorry
-      --exact TypedExpr.WellTyped.lit (Prim.WellTyped.entityUID uid h₄)
+      exact TypedExpr.WellTyped.lit (Prim.WellTyped.entityUID uid h₄)
     · cases h₃
 
 theorem typechecked_is_well_typed_after_lifting_var {v : Var} {c₁ c₂ : Capabilities} {env : Environment} {ty : TypedExpr} {request : Request} {entities : Entities} :
@@ -59,15 +59,18 @@ theorem typechecked_is_well_typed_after_lifting_var {v : Var} {c₁ c₂ : Capab
   TypedExpr.WellTyped env ty.liftBoolTypes
 := by
   intro h₁ h₂ h₃
-  simp only [typeOf, typeOfVar, List.empty_eq, Function.comp_apply, ok] at h₃
+  simp only [typeOf, typeOfVar] at h₃
   split at h₃ <;>
-  simp at h₃ <;>
-  rcases h₃ with ⟨h₃, _⟩ <;>
-  simp [← h₃, TypedExpr.liftBoolTypes, CedarType.liftBoolTypes]
-  · exact TypedExpr.WellTyped.var (Var.WellTyped.principal)
-  · exact TypedExpr.WellTyped.var (Var.WellTyped.action)
-  · exact TypedExpr.WellTyped.var (Var.WellTyped.resource)
-  · sorry
+  simp only [List.empty_eq, Function.comp_apply] at h₃ <;>
+  rcases h₃ with ⟨h₃, _⟩
+  · simp only [TypedExpr.liftBoolTypes, CedarType.liftBoolTypes]
+    exact TypedExpr.WellTyped.var (Var.WellTyped.principal)
+  · simp only [TypedExpr.liftBoolTypes, CedarType.liftBoolTypes]
+    exact TypedExpr.WellTyped.var (Var.WellTyped.action)
+  · simp only [TypedExpr.liftBoolTypes, CedarType.liftBoolTypes]
+    exact TypedExpr.WellTyped.var (Var.WellTyped.resource)
+  · simp only [TypedExpr.liftBoolTypes]
+    exact TypedExpr.WellTyped.var (Var.WellTyped.context)
 
 theorem well_typed_is_sound_lit
 {v : Value}
@@ -122,6 +125,6 @@ InstanceOfType v (TypedExpr.var var ty).typeOf
     exact InstanceOfType.instance_of_entity env.reqty.action env.reqty.action.ty this
   case context =>
     rcases h₁ with ⟨⟨_, _, _, h₁⟩, _, _⟩
-    exact h₁
+    exact type_lifting_preserves_instance_of_type h₁
 
 end Cedar.Thm
